git/Augustindou/natural2lean-lean-project-template/examples/in-progress/sum-over-i/theorem.lean
@@ -1,0 +1,30 @@
+import LeanUtils
+open Nat
+
+theorem n_cube_plus_2_n (n : Nat) : divisible 3 (n^3 + 2*n) := by
+  match n with
+  | 0 => trivial
+  | k+1 => 
+    have h₁ : divisible 3 (k ^ 3 + 2 * k) := n_cube_plus_2_n k
+    
+    have ⟨z, h₂⟩ : ∃ z, k^3 + 2*k = 3*z := by simp_all
+    
+    have h₃ : (k + 1) ^ 3 + 2 * (k + 1) = 3*(z + k^2 + k + 1) := by
+      calc
+        (k + 1) ^ 3 + 2 * (k + 1) = k^3 + 3*k^2 + 5*k + 3 := by 
+          try simp_all
+          try ring
+        _ = k^3 + 2*k + 3 * (k^2 + k + 1) := by 
+          admit
+        _ = 3*z + 3 * (k^2 + k + 1) := by
+          try simp_all
+          try ring
+        _ = 3 * (z + k^2 + k + 1) := by
+          try simp_all
+          try ring
+    
+    rw [divisible]
+
+    exact ⟨_, by admit⟩
+    
+
