git/cruhland/lean4-axiomatic/Lean4Axiomatic/Integer.lean
@@ -1,6 +1,7 @@
 import Lean4Axiomatic.Integer.Addition
 import Lean4Axiomatic.Integer.Core
 import Lean4Axiomatic.Integer.Multiplication
+import Lean4Axiomatic.Integer.Negation
 
 /-!
 # Combined typeclass of all integer definitions and properties
@@ -8,30 +9,45 @@ import Lean4Axiomatic.Integer.Multiplication
 
 namespace Lean4Axiomatic
 
-open Integer (Addition.Base Core Equality Multiplication.Base)
+open Integer (
+  Addition.Base Conversion Equality Multiplication.Base Negation.Base
+)
 
 /--
 The class of [integers](https://en.wikipedia.org/wiki/Integer).
 
-The fields of this class express many integer properties. Any type `α` for
-which an instance of `Integer α` exists must obey all of them. However, most of
-the properties can be derived from a few essential ones, reducing the work
-required to construct an instance.
+It is parameterized not only on a type `ℤ` that must satisfy the properties of
+integers, but also on a type `ℕ` that obeys the properties of natural numbers
+(via `Natural ℕ`). This is to support the crucial fact that a bijection exists
+between the natural numbers and the nonnegative integers (provided by
+`Integer.Conversion.from_natural`).
+
+Although there are many integer properties expressed by this class, most of
+them can be derived from a few essential ones, reducing the work required to
+construct an instance.
 
 **Named parameters**
-- `ℤ`: a type that obeys all of the properties provided by this class.
+- `ℕ`: A type that obeys all of the properties of the natural numbers.
+- `ℤ`: A type that obeys all of the properties provided by this class.
+
+**Class parameters**
+- `Natural ℕ`: Evidence that `ℕ` implements the natural numbers.
 -/
-class Integer (ℤ : Type) :=
-  toCore : Core ℤ
+class Integer (ℕ : Type) [Natural ℕ] (ℤ : Type) :=
+  toEquality : Equality ℤ
+  toConversion : Conversion ℕ ℤ
   toAddition : Addition.Base ℤ
+  toNegation : Negation.Base ℤ
   toMultiplication : Multiplication.Base ℤ
 
 namespace Integer
 
-attribute [instance] toCore
+attribute [instance] toConversion
+attribute [instance] toEquality
 
 export Addition (addOp)
 export Equality (eqvOp)
 export Multiplication (mulOp)
+export Negation (negOp)
 
 end Lean4Axiomatic.Integer
