git/cruhland/lean4-axiomatic/Lean4Axiomatic/Integer/Core.lean
@@ -1,3 +1,4 @@
+import Lean4Axiomatic.Natural
 import Lean4Axiomatic.Relation.Equivalence
 
 /-!
@@ -10,7 +11,7 @@ namespace Lean4Axiomatic.Integer
 Definitions pertaining to equality of integer values.
 
 **Named parameters**
-- `ℤ`: the type of integers.
+- `ℤ`: The type of integers.
 -/
 class Equality (ℤ : Type) :=
   /-- The equality relation on integers, expressed with the syntax `a ≃ b`. -/
@@ -19,12 +20,19 @@ class Equality (ℤ : Type) :=
 attribute [instance] Equality.eqvOp
 
 /--
-Packages together the basic properties of integers, to reduce the amount of
-class references needed for more advanced properties.
+Definitions pertaining to conversion of other types into or out of integers.
 
 **Named parameters**
-- `ℤ`: the type of integers.
+- `ℕ`: A type that implements the natural numbers.
+- `ℤ`: The type of integers.
+
+**Class parameters**
+- `Natural ℕ`: Evidence that `ℕ` implements the natural numbers.
 -/
-class Core (ℤ : Type) extends Equality ℤ
+class Conversion (ℕ : Type) [Natural ℕ] (ℤ : Type) :=
+  /-- Every natural number has an integer representation. -/
+  from_natural : Coe ℕ ℤ
+
+attribute [instance] Conversion.from_natural
 
 end Lean4Axiomatic.Integer
