git/cruhland/lean4-axiomatic/Lean4Axiomatic/Integer/Negation.lean
@@ -1,0 +1,35 @@
+import Lean4Axiomatic.AbstractAlgebra
+import Lean4Axiomatic.Integer.Core
+
+namespace Lean4Axiomatic.Integer
+
+/-!
+# Definition and properties of integer negation and subtraction
+-/
+
+/--
+Definition of negation, and properties that it must satisfy.
+
+All other properties of negation can be derived from these.
+
+**Named parameters**
+- `ℤ`: The type of integers.
+
+**Class parameters**
+- `Equality ℤ`: Required to express most properties of negation.
+-/
+class Negation.Base (ℤ : Type) [Equality ℤ] :=
+  /-- Definition of and syntax for negation. -/
+  negOp : Neg ℤ
+
+  /--
+  Negation preserves equality of integers; two equal integers are still equal
+  after both are negated.
+  -/
+  neg_substitutive : AA.Substitutive₁ (α := ℤ) (-·) (· ≃ ·) (· ≃ ·)
+
+namespace Negation
+export Negation.Base (negOp)
+end Negation
+
+end Lean4Axiomatic.Integer
