git/xubaiw/Dta.lean/Dta/Float.lean
@@ -1,0 +1,9 @@
+namespace Dta
+
+@[extern c inline "(double)(#1)"]
+opaque uint16ToFloat : UInt16 → Float
+
+@[extern c inline "(double)(#1)"]
+opaque uint32ToDouble : UInt32 → Float
+
+end Dta
