git/xubaiw/Dta.lean/Dta/Parser.lean
@@ -1,9 +1,46 @@
 import Dta.Basic
+import Dta.Float
 import Parsec
 
 open Parsec ByteArrayParser
 
 namespace Dta
+
+def wrapped (tag : String) (p : ByteArrayParser α) : ByteArrayParser α := do
+  expectS s!"<{tag}>"
+  let s ← p
+  expectS s!"</{tag}>"
+  return s
+
+def wrappedArray (tag : String) (num : Nat) (p : ByteArrayParser α) : ByteArrayParser (Array α) := do
+  wrapped tag (readArray num p)
+
+def wrappedArrayString (tag : String) (num length : Nat) (f : String → String := (·.replace "\x00" "")) : ByteArrayParser (Array String) := do
+  wrappedArray tag num s
+where
+  s := do
+    let s ← readString length
+    return f s
+
+@[inline]
+partial def manyCore (p : ByteArrayParser α) (acc : Array α) : ByteArrayParser (Array α) := do
+  try
+    let res ← p
+    manyCore p (acc.push res)
+  catch _ =>
+    return acc
+
+@[inline]
+def many (p : ByteArrayParser α) : ByteArrayParser $ Array α := manyCore p #[]
+
+partial def readString' : ByteArrayParser String := do
+  let mut arr := ByteArray.empty
+  repeat do
+    let s ← peek
+    if s = 0 then
+      break
+    arr := arr.push s
+  return arr |> String.fromUTF8Unchecked
 
 def release : ByteArrayParser Release := do
   match ←readString 3 with
@@ -51,34 +88,17 @@ def timestamp? : ByteArrayParser (Option String) := do
   | 17 => return (←readString 17)
   |  _ => error "length of timestamp must be 0 or 17"
 
-def header : ByteArrayParser Header := do
-  expectS "<header>"
-  expectS "<release>"
-  let r ← release
-  expectS "</release>"
-  expectS "<byteorder>"
-  let e ← byteorder
-  expectS "</byteorder>"
-  expectS "<K>"
-  let k ← k r e
-  expectS "</K>"
-  expectS "<N>"
-  let n ← n e
-  expectS "</N>"
-  expectS "<label>"
-  let label ← label e
-  expectS "</label>"
-  expectS "<timestamp>"
-  let timestamp? ← timestamp?
-  expectS "</timestamp>"
-  expectS "</header>"
+def header : ByteArrayParser Header := wrapped "header" do
+  let r ← wrapped "release" release
+  let e ← wrapped "byteorder" byteorder
+  let k ← wrapped "K" (k r e)
+  let n ← wrapped "N" (n e)
+  let label ← wrapped "label" (label e)
+  let timestamp? ← wrapped "timestamp" timestamp?
   return ⟨r, e, k, n, label, timestamp?⟩
 
 def map (e : Byteorder) : ByteArrayParser Map := do
-  expectS "<map>"
-  let map ← readArray 14 <| read64 e
-  expectS "</map>"
-  return map
+  wrappedArray "map" 14 (read64 e)
 
 def variableTypes (k : typeK r) (e : Byteorder) : ByteArrayParser VariableTypes := do
   expectS "<variable_types>"
@@ -100,31 +120,61 @@ def variableTypes (k : typeK r) (e : Byteorder) : ByteArrayParser VariableTypes 
   expectS "</variable_types>"
   return arr
 
--- def readBytes (sz : Nat) : ByteArrayParser ByteArray := do
---   let pos ← get
---   let ba ← read
---   if pos + sz <= ba.size then
---     (pure <| ba.extract pos (pos + sz)) <* modify (· + sz)
---   else
---     error s!"eof before {sz} bytes"
+def varnames (k : typeK r) : ByteArrayParser VarNames :=
+  wrappedArrayString "varnames" k.toNat 129
 
-def varname : ByteArrayParser String := do
-  let s ← readString 129
-  return s.replace "\x00" ""
+def sortlist (k : typeK r) (e : Byteorder) : ByteArrayParser SortList := do
+  wrappedArray "sortlist" (k.toNat + 1) (read16 e)
 
-def varnames (k : typeK r) : ByteArrayParser VarNames := do
-  expectS "<varnames>"
-  let varnames ← readArray k.toNat varname
-  expectS "</varnames>"
-  return varnames
+def formats (k : typeK r) : ByteArrayParser Formats :=
+  wrappedArrayString "formats" k.toNat 57
+
+def valueLabelNames (k : typeK r) : ByteArrayParser ValueLabelNames :=
+  wrappedArrayString "value_label_names" k.toNat 129
+
+def variableLabels (k : typeK r) : ByteArrayParser VariableLabels := 
+  wrappedArrayString "variable_labels" k.toNat 321 λ s => if s.startsWith "\x00" then "" else s.replace "\x00" ""
+
+def characteristic (e : Byteorder) : ByteArrayParser Characteristic := wrapped "ch" do
+  let _length ← read32 e
+  let varname ← readString 129
+  let charname ← readString 129
+  let contents ← many readString'
+  return ⟨varname, charname, contents⟩
+
+def characteristics (e : Byteorder) : ByteArrayParser Characteristics := wrapped "characteristics" (many (characteristic e))
+
+def observation (e : Byteorder) (k : typeK r) (ty : VariableType) : ByteArrayParser Observation := do
+  let p : ByteArrayParser (ty.toLeanType) := match ty with
+  | .str n => readString n.val
+  | .strL => sorry
+  | .double => read32 e |>.map uint32ToDouble
+  | .float => read16 e |>.map uint16ToFloat
+  | .long => read32 e
+  | .int => read16 e
+  | .byte => read8
+  sorry
+
+def data (e : Byteorder) (k : typeK r) (varTypes : VariableTypes) : ByteArrayParser Data := wrapped "data" do
+  let mut obs := #[]
+  for ty in varTypes do
+    obs := obs.push (←observation k ty)
+  return obs
 
 def dta : ByteArrayParser Dta := do
   expectS "<stata_dta>"
   let header ← header
-  let map ← map header.byteorder
-  let varTypes ← variableTypes header.k header.byteorder
-  let varnames ← varnames header.k
+  let {k, byteorder := e, ..} := header
+  let map ← map e
+  let varTypes ← variableTypes k e
+  let varnames ← varnames k
+  let sortlist ← sortlist k e
+  let formats ← formats k
+  let valueLabelNames ← valueLabelNames k
+  let variableLabels ← variableLabels k
+  let characteristics ← characteristics e
+  let data ← data e k varTypes
   -- expectS "</stata_dta>"
-  return ⟨header, map, varTypes, varnames⟩
+  return ⟨header, map, varTypes, varnames, sortlist, formats, valueLabelNames, variableLabels, characteristics, data⟩
 
 end Dta
